move to scoped syntax

tests/utlc.sig
@@ -1,0 +1,4 @@
+term : Type
+
+app  : term -> term -> term
+lam  : (bind term in term) -> term
