theories/LevelOne.v
@@ -1,3 +1,4 @@
+From Coq Require Import Program.Equality.
 From Prototype Require Import Prelude Sig.
 
 (** This file defines terms and substitutions over an abstract signature.
@@ -12,122 +13,131 @@ Definition arg_ty := @Sig.arg_ty (Sig.base sig).
 (** *** Terms. *)
 (*********************************************************************************)
 
-(** Terms are indexed by (meta-level) sorts. 
-    This is a trick to avoid encoding terms as a mutual inductive,
-    and seems to be easier to work with. *)
-Inductive sort := 
-| T (* Term. *)
-| A (a : arg_ty) (* Argument. *)
-| AL (args : list arg_ty). (* Argument list. *)
+(** Terms are indexed by (meta-level) kinds. *)
+Inductive kind := 
+| (** Term. *)
+  K_t : kind
+| (** Constructor argument. *)
+  K_a : arg_ty -> kind
+| (** List of constructor arguments. *)
+  K_al : list arg_ty -> kind.
 
-(** Terms over an abstract signature. *)
-Inductive term : sort -> Type :=
-(** Terms. *)
-| (* A term variable. *)
-  T_var : nat -> term T
-| (* A _non-variable_ term constructor, applied to a list of arguments. *)
-  T_ctor : forall c, term (AL (Sig.ctor_type sig c)) -> term T
-(** An argument list, of type [tys]. *)
-| AL_nil : term (AL [])
-| AL_cons {ty tys} : term (A ty) -> term (AL tys) -> term (AL (ty :: tys))
-(** A single argument of type [ty]. *)
-| A_base : forall b, Sig.denote_base sig b -> term (A (AT_base b))
-| A_term : term T -> term (A AT_term)
-| A_bind {ty} : term (A ty) -> term (A (AT_bind ty)).
+(** Terms over an abstract signature. 
+    Terms are indexed by a scope (an integer) and a kind. *)
+Inductive term : nat -> kind -> Type :=
+| (** Term variable. *)
+  T_var {n} : fin n -> term n K_t
+| (** Non-variable term constructor, applied to a list of arguments. *)
+  T_ctor {n} : forall c, term n (K_al (Sig.ctor_type sig c)) -> term n K_t
+| (** Empty argument list. *)
+  AL_nil {n} : term n (K_al [])
+| (** Non-empty argument list. *)
+  AL_cons {n ty tys} : term n (K_a ty) -> term n (K_al tys) -> term n (K_al (ty :: tys))
+| (** Base argument (e.g. bool or string). *)
+  A_base {n} : forall b, Sig.denote_base sig b -> term n (K_a (AT_base b))
+| (** Term argument. *)
+  A_term {n} : term n K_t -> term n (K_a AT_term)
+| (** Binder argument. *)
+  A_bind {n ty} : term (S n) (K_a ty) -> term n (K_a (AT_bind ty)).
 
 (*********************************************************************************)
 (** *** Renamings. *)
 (*********************************************************************************)
 
-(** A renaming on terms is a function [nat -> nat] which is applied
+(** A renaming on terms is a function [fin n -> fin m] which is applied
     to all free variables. *)
-Definition ren := nat -> nat.
+Definition ren n m := fin n -> fin m.
 
 (** The identity renaming. *)
-Definition rid : ren := fun n => n.
+Definition rid {n} : ren n n := 
+  fun i => i.
 
 (** [rshift k] shifts indices by [k]. *)
-Definition rshift (k : nat) : ren := fun n => n + k.
+Definition rshift {n} (k : nat) : ren n (k + n) := 
+  fun i => fin_weaken k i.
 
 (** Cons an index with a renaming. *)
-Definition rcons (n0 : nat) (r : ren) : ren :=
-  fun n =>
-    match n with 
-    | 0 => n0
-    | S n => r n
-    end.
-#[global] Instance rcons_notation : Scons nat ren :=
-{ gen_scons := rcons }.
+Definition rcons {n m} (i0 : fin m) (r : ren n m) : ren (S n) m :=
+  fun i =>
+    match i in fin (S n0) return ren n0 m -> fin m with 
+    | fin_zero => fun _ => i0
+    | fin_succ i => fun r => r i
+    end r.
+#[global] Instance rcons_notation n m : Scons (fin m) (ren n m) (ren (S n) m) :=
+{ gen_scons := @rcons n m }.
 
-(** Compose two renamings (right to left composition). *)
-Definition rcomp (r1 r2 : ren) : ren :=
-  fun n => r1 (r2 n).
-#[global] Instance rcomp_notation : Scomp ren :=
+(** Compose two renamings (left to right composition). *)
+Definition rcomp {n m o} (r1 : ren n m) (r2 : ren m o) : ren n o :=
+  fun i => r2 (r1 i).
+#[global] Instance rcomp_notation {n m o} : Scomp (ren n m) (ren m o) (ren n o) :=
 { gen_scomp := rcomp }.
 
 (** Lift a renaming through a binder. *)
-Definition up_ren (r : ren) : ren := 0 .: rshift 1 ∘ r.
+Definition up_ren {n m} (r : ren n m) : ren (S n) (S m) := 
+  fin_zero .: r >> rshift 1.
  
 (** Rename a term. *)
-Fixpoint rename {so} (t : term so) (r : ren) : term so :=
-  match t with 
-  | T_var n => T_var (r n)
-  | T_ctor c args => T_ctor c (rename args r)
-  | AL_nil => AL_nil
-  | AL_cons a args => AL_cons (rename a r) (rename args r)
-  | A_base b x => A_base b x
-  | A_term t => A_term (rename t r)
-  | A_bind a => A_bind (rename a (up_ren r))
+Fixpoint rename {n m} {k} (t : term n k) (r : ren n m) : term m k :=
+  match t, r with 
+  | T_var i, r => T_var (r i)
+  | T_ctor c args, r => T_ctor c (rename args r)
+  | AL_nil, r => AL_nil
+  | AL_cons a args, r => AL_cons (rename a r) (rename args r)
+  | A_base b x, r => A_base b x
+  | A_term t, r => A_term (rename t r)
+  | A_bind a, r => A_bind (rename a (up_ren r))
   end.
-#[global] Instance rename_notation so : Subst (term so) ren :=
+#[global] Instance rename_notation n m k : Subst (term n k) (ren n m) (term m k) :=
 { gen_subst := rename }.
   
 (*********************************************************************************)
 (** *** Substitutions. *)
 (*********************************************************************************)
 
-(** A substitution on terms is a function [nat -> term T] which is applied 
+(** A substitution on terms is a function [fin n -> term m K_t] which is applied 
     to all free variables. *)
-Definition subst := nat -> term T.
+Definition subst n m := fin n -> term m K_t.
 
 (** The identity substitution. *)
-Definition sid : subst := fun n => T_var n.
+Definition sid {n} : subst n n := 
+  fun i => T_var i.
 
 (** [sshift k] shifts indices by [k]. *)
-Definition sshift (k : nat) : subst := fun n => T_var (n + k).
+Definition sshift {n} (k : nat) : subst n (k + n) := 
+  fun i => T_var (fin_weaken k i).
 
 (** Cons a term with a substitution. *)
-Definition scons (t : term T) (s : subst) : subst :=
-  fun n => 
-    match n with 
-    | 0 => t
-    | S n => s n
-    end.
-#[global] Instance scons_notation : Scons (term T) subst :=
+Definition scons {n m} (t : term m K_t) (s : subst n m) : subst (S n) m :=
+  fun i => 
+    match i in fin (S n0) return subst n0 m -> term m K_t with 
+    | fin_zero => fun _ => t
+    | fin_succ i => fun s => s i
+    end s.
+#[global] Instance scons_notation n m : Scons (term m K_t) (subst n m) (subst (S n) m) :=
 { gen_scons := scons }.
 
 (** Lift a substitution through a binder. *)
-Definition up_subst (s : subst) : subst :=
-  T_var 0 .: (fun n => rename (s n) (rshift 1)).
+Definition up_subst {n m} (s : subst n m) : subst (S n) (S m) :=
+  T_var fin_zero .: (fun i => (s i)[: rshift 1]).
 
 (** Apply a substitution to a term. *)
-Fixpoint substitute {so} (t : term so) (s : subst) : term so :=
-  match t with 
-  | T_var n => s n
-  | T_ctor c args => T_ctor c (substitute args s)
-  | AL_nil => AL_nil
-  | AL_cons a args => AL_cons (substitute a s) (substitute args s)
-  | A_base b x => A_base b x
-  | A_term t => A_term (substitute t s)
-  | A_bind a => A_bind (substitute a (up_subst s))
+Fixpoint substitute {n m} {k} (t : term n k) (s : subst n m) : term m k :=
+  match t, s with 
+  | T_var n, s => s n
+  | T_ctor c args, s => T_ctor c (substitute args s)
+  | AL_nil, s => AL_nil
+  | AL_cons a args, s => AL_cons (substitute a s) (substitute args s)
+  | A_base b x, s => A_base b x
+  | A_term t, s => A_term (substitute t s)
+  | A_bind a, s => A_bind (substitute a (up_subst s))
   end.
-#[global] Instance substitute_notation so : Subst (term so) subst :=
+#[global] Instance substitute_notation n m k : Subst (term n k) (subst n m) (term m k) :=
 { gen_subst := substitute }.
 
-(** Composition of substitutions (right to left). *)
-Definition scomp (s1 s2 : subst) : subst :=
-  fun n => substitute (s2 n) s1.
-#[global] Instance scomp_notation : Scomp subst :=
+(** Left to right composition of substitutions. *)
+Definition scomp {n m o} (s1 : subst n m) (s2 : subst m o) : subst n o :=
+  fun i => (s1 i)[: s2].
+#[global] Instance scomp_notation n m o : Scomp (subst n m) (subst m o) (subst n o) :=
 { gen_scomp := scomp }.
 
 (*********************************************************************************)
@@ -138,120 +148,115 @@ Definition scomp (s1 s2 : subst) : subst :=
 Definition point_eq {A B} : relation (A -> B) := pointwise_relation _ eq.
 Notation "f =₁ g" := (point_eq f g) (at level 75).
 
-#[global] Instance up_ren_proper : Proper (point_eq ==> point_eq) up_ren.
+#[global] Instance up_ren_proper n m : Proper (point_eq ==> point_eq) (@up_ren n m).
 Proof. 
-intros r1 r2 Hr [|n] ; cbv [up_ren] ; simpl.
+intros r1 r2 Hr i. dependent destruction i ; cbv [up_ren] ; simpl.
 - reflexivity.
 - cbv [rcomp rshift]. auto.
 Qed. 
 
-#[global] Instance rename_proper so :
-  Proper (eq ==> point_eq ==> eq) (@rename so).
+#[global] Instance rename_proper n m k :
+  Proper (eq ==> point_eq ==> eq) (@rename n m k).
 Proof.
-intros t ? <-. induction t ; intros s1 s2 Hs ; simpl ; try (now auto).
-f_equal. apply IHt. now rewrite Hs.
+intros t ? <-. revert m. 
+induction t ; intros m s1 s2 Hs ; simpl ; try (now auto).
+- specialize (IHt m). auto.
+- specialize (IHt1 m). specialize (IHt2 m). auto.
+- specialize (IHt m). auto.
+- f_equal. apply IHt. now rewrite Hs.
 Qed.
 
-#[global] Instance up_subst_proper : Proper (point_eq ==> point_eq) up_subst.
+#[global] Instance up_subst_proper n m : Proper (point_eq ==> point_eq) (@up_subst n m).
 Proof.
-intros s1 s2 Hs [|n] ; cbv [up_subst] ; simpl.
+intros s1 s2 Hs i. dependent destruction i ; cbv [up_subst] ; simpl.
 - reflexivity.
 - now rewrite Hs.
 Qed. 
 
-#[global] Instance substitute_proper so : 
-  Proper (eq ==> point_eq ==> eq) (@substitute so).
+#[global] Instance substitute_proper n m k : 
+  Proper (eq ==> point_eq ==> eq) (@substitute n m k).
 Proof. 
-intros t ? <-. induction t ; intros s1 s2 Hs ; simpl ; try (now auto).
-f_equal. apply IHt. now rewrite Hs.
+intros t ? <-. revert m. induction t ; intros m s1 s2 Hs ; simpl ; try (now auto).
+- specialize (IHt m). auto.
+- specialize (IHt1 m). specialize (IHt2 m). auto.
+- specialize (IHt m). auto.
+- f_equal. apply IHt. now rewrite Hs.
 Qed. 
 
 (*********************************************************************************)
 (** *** Properties of substitution. *)
 (*********************************************************************************)
 
-Lemma rshift1 n : rshift 1 n = S n.
-Proof. cbv [rshift]. lia. Qed.
+(*Lemma rshift1 n (i : fin n) : rshift 1 i = fin_succ i.
+Proof. cbv [rshift]. simpl. reflexivity. Qed.*)
 
-Lemma up_ren_comp r1 r2 : 
-  up_ren r1 ∘ up_ren r2 =₁ up_ren (r1 ∘ r2).
-Proof.
-intros [|n] ; simpl.
-- reflexivity.
-- cbv [rcomp up_ren]. simpl. cbv [rcomp rcons].
-  repeat rewrite rshift1. reflexivity.
-Qed.
+Lemma up_ren_comp {n m o} (r1 : ren n m) (r2 : ren m o) : 
+  up_ren r1 >> up_ren r2 =₁ up_ren (r1 >> r2).
+Proof. intros i. dependent destruction i ; reflexivity. Qed.
 
-Lemma ren_ren so (t : term so) (r1 r2 : ren) : 
-  t[: r1][: r2] = t[: r2 ∘ r1].
+Lemma ren_ren {n m o k} (t : term n k) (r1 : ren n m) (r2 : ren m o) : 
+  t[: r1][: r2] = t[: r1 >> r2].
 Proof.
-revert r1 r2. induction t ; intros r1 r2 ; simpl ; try (now auto).
+revert m o r1 r2. induction t ; intros m o r1 r2 ; simpl ; try (now auto).
 - now setoid_rewrite IHt.
 - setoid_rewrite IHt1. now setoid_rewrite IHt2.
 - now setoid_rewrite IHt.
 - setoid_rewrite IHt. now rewrite up_ren_comp.
 Qed.
 
-Lemma subst_ren so (t : term so) (s : subst) (r : ren) : 
+Lemma subst_ren {n m o k} (t : term n k) (s : subst n m) (r : ren m o) : 
   t[: s][: r] = t[: fun n => (s n)[: r]].
 Proof.
-revert s r. induction t ; intros s r ; simpl ; try (now auto).
+revert m o s r. induction t ; intros m o s r ; simpl ; try (now auto).
 - now setoid_rewrite IHt.
 - setoid_rewrite IHt1. now setoid_rewrite IHt2.
 - now setoid_rewrite IHt.
 - f_equal. setoid_rewrite IHt. apply substitute_proper ; [reflexivity|].
-  intros [|n] ; simpl ; [reflexivity|].
+  intros i ; dependent destruction i ; simpl ; [reflexivity|].
   cbv [up_subst]. simpl. repeat setoid_rewrite ren_ren.
-  apply rename_proper ; [reflexivity|].
-  intros [|n'] ; simpl ; [reflexivity|].
-  cbv [rcomp up_ren]. simpl. repeat rewrite rshift1. cbv [rcomp].
-  rewrite rshift1. reflexivity.
+  apply rename_proper ; reflexivity.
 Qed.
 
-Lemma ren_subst so (t : term so) (s : subst) (r : ren) : 
+Lemma ren_subst {n m o k} (t : term n k) (r : ren n m) (s : subst m o) : 
   t[: r][: s] = t[: fun n => s (r n)].
 Proof.
-revert s r. induction t ; intros s r ; simpl ; try (now auto).
+revert m o s r. induction t ; intros m o s r ; simpl ; try (now auto).
 - now setoid_rewrite IHt. 
 - setoid_rewrite IHt1. now setoid_rewrite IHt2.
 - now setoid_rewrite IHt.
 - f_equal. setoid_rewrite IHt. apply substitute_proper ; [reflexivity|].
-  intros [|n] ; simpl ; [reflexivity|].
-  cbv [up_subst up_ren]. simpl. cbv [scons rcomp].
-  rewrite rshift1. reflexivity.
+  intros i ; dependent destruction i ; reflexivity.
 Qed.  
 
-Lemma subst_subst so (t : term so) (s1 s2 : subst) : 
-  t[: s1][: s2] = t[: s2 ∘ s1].
+Lemma subst_subst {n m o k} (t : term n k) (s1 : subst n m) (s2 : subst m o) : 
+  t[: s1][: s2] = t[: s1 >> s2].
 Proof.
-revert s1 s2. induction t ; intros s1 s2 ; cbn ; try (now auto).
+revert m o s1 s2. induction t ; intros m o s1 s2 ; cbn ; try (now auto).
 - now setoid_rewrite IHt.
 - setoid_rewrite IHt1. setoid_rewrite IHt2. reflexivity.
 - now setoid_rewrite IHt.
-- f_equal. setoid_rewrite IHt. apply substitute_proper ; [auto | simpl].
-  intros [|n] ; simpl ; [reflexivity|].
-  cbv [scomp]. simpl. 
-  setoid_rewrite subst_ren. setoid_rewrite ren_subst. simpl.
-  apply substitute_proper ; [reflexivity|].
-  intros n'. rewrite rshift1. reflexivity.
+- f_equal. setoid_rewrite IHt. apply substitute_proper ; [reflexivity | simpl].
+  intros i ; dependent destruction i ; simpl ; [reflexivity|].
+  cbv [scomp]. simpl. setoid_rewrite subst_ren. setoid_rewrite ren_subst. reflexivity.
 Qed.
 
-Lemma up_subst_sid : (up_subst sid) =₁ sid.
-Proof. intros [|n] ; cbv [up_subst rshift] ; simpl ; auto. Qed. 
+Lemma up_subst_sid {n} : (up_subst (@sid n)) =₁ sid.
+Proof. intros i ; dependent destruction i ; reflexivity. Qed.
 
-Lemma subst_sid so (t : term so) : t[: sid] = t.
+Lemma subst_sid {n k} (t : term n k) : t[: sid] = t.
 Proof.
 induction t ; try (now auto).
 simpl. rewrite up_subst_sid. now setoid_rewrite IHt.
 Qed.
 
-Lemma scomp_id_l s : sid ∘ s =₁ s.
-Proof. intros n. simpl. cbv [scomp]. now setoid_rewrite subst_sid. Qed.
-    
-Lemma scomp_id_r s : s ∘ sid =₁ s.
-Proof. intros n. simpl. cbv [scomp]. simpl. reflexivity. Qed.
+Lemma scomp_id_l {n m} (s : subst n m) : sid >> s =₁ s.
+Proof. reflexivity. Qed.
 
-Lemma scomp_assoc (s1 s2 s3 : subst) : (s1 ∘ s2) ∘ s3 =₁ s1 ∘ (s2 ∘ s3).
-Proof. intros n. simpl. cbv [scomp]. now setoid_rewrite subst_subst. Qed.
+Lemma scomp_id_r {n m} (s : subst n m) : s >> sid =₁ s.
+Proof. intros i. simpl. cbv [scomp]. now setoid_rewrite subst_sid. Qed.    
+
+Lemma scomp_assoc {n m o p} (s1 : subst n m) (s2 : subst m o) (s3 : subst o p) : 
+  (s1 >> s2) >> s3 =₁ s1 >> (s2 >> s3).
+Proof. intros i. simpl. cbv [scomp]. now setoid_rewrite subst_subst. Qed.
 
 End WithSig.
