tests/utlc.v
@@ -1,0 +1,745 @@
+Require Import core fintype.
+
+Require Import Setoid Morphisms Relation_Definitions.
+
+
+Module Core.
+
+Inductive term (n_term : nat) : Type :=
+  | var_term : fin n_term -> term n_term
+  | app : term n_term -> term n_term -> term n_term
+  | lam : term (S n_term) -> term n_term.
+
+Lemma congr_app {m_term : nat} {s0 : term m_term} {s1 : term m_term}
+  {t0 : term m_term} {t1 : term m_term} (H0 : s0 = t0) (H1 : s1 = t1) :
+  app m_term s0 s1 = app m_term t0 t1.
+Proof.
+exact (eq_trans (eq_trans eq_refl (ap (fun x => app m_term x s1) H0))
+         (ap (fun x => app m_term t0 x) H1)).
+Qed.
+
+Lemma congr_lam {m_term : nat} {s0 : term (S m_term)} {t0 : term (S m_term)}
+  (H0 : s0 = t0) : lam m_term s0 = lam m_term t0.
+Proof.
+exact (eq_trans eq_refl (ap (fun x => lam m_term x) H0)).
+Qed.
+
+Lemma upRen_term_term {m : nat} {n : nat} (xi : fin m -> fin n) :
+  fin (S m) -> fin (S n).
+Proof.
+exact (up_ren xi).
+Defined.
+
+Lemma upRen_list_term_term (p : nat) {m : nat} {n : nat}
+  (xi : fin m -> fin n) : fin (plus p m) -> fin (plus p n).
+Proof.
+exact (upRen_p p xi).
+Defined.
+
+Fixpoint ren_term {m_term : nat} {n_term : nat}
+(xi_term : fin m_term -> fin n_term) (s : term m_term) {struct s} :
+term n_term :=
+  match s with
+  | var_term _ s0 => var_term n_term (xi_term s0)
+  | app _ s0 s1 => app n_term (ren_term xi_term s0) (ren_term xi_term s1)
+  | lam _ s0 => lam n_term (ren_term (upRen_term_term xi_term) s0)
+  end.
+
+Lemma up_term_term {m : nat} {n_term : nat} (sigma : fin m -> term n_term) :
+  fin (S m) -> term (S n_term).
+Proof.
+exact (scons (var_term (S n_term) var_zero) (funcomp (ren_term shift) sigma)).
+Defined.
+
+Lemma up_list_term_term (p : nat) {m : nat} {n_term : nat}
+  (sigma : fin m -> term n_term) : fin (plus p m) -> term (plus p n_term).
+Proof.
+exact (scons_p p (funcomp (var_term (plus p n_term)) (zero_p p))
+         (funcomp (ren_term (shift_p p)) sigma)).
+Defined.
+
+Fixpoint subst_term {m_term : nat} {n_term : nat}
+(sigma_term : fin m_term -> term n_term) (s : term m_term) {struct s} :
+term n_term :=
+  match s with
+  | var_term _ s0 => sigma_term s0
+  | app _ s0 s1 =>
+      app n_term (subst_term sigma_term s0) (subst_term sigma_term s1)
+  | lam _ s0 => lam n_term (subst_term (up_term_term sigma_term) s0)
+  end.
+
+Lemma upId_term_term {m_term : nat} (sigma : fin m_term -> term m_term)
+  (Eq : forall x, sigma x = var_term m_term x) :
+  forall x, up_term_term sigma x = var_term (S m_term) x.
+Proof.
+exact (fun n =>
+       match n with
+       | Some fin_n => ap (ren_term shift) (Eq fin_n)
+       | None => eq_refl
+       end).
+Qed.
+
+Lemma upId_list_term_term {p : nat} {m_term : nat}
+  (sigma : fin m_term -> term m_term)
+  (Eq : forall x, sigma x = var_term m_term x) :
+  forall x, up_list_term_term p sigma x = var_term (plus p m_term) x.
+Proof.
+exact (fun n =>
+       scons_p_eta (var_term (plus p m_term))
+         (fun n => ap (ren_term (shift_p p)) (Eq n)) (fun n => eq_refl)).
+Qed.
+
+Fixpoint idSubst_term {m_term : nat} (sigma_term : fin m_term -> term m_term)
+(Eq_term : forall x, sigma_term x = var_term m_term x) (s : term m_term)
+{struct s} : subst_term sigma_term s = s :=
+  match s with
+  | var_term _ s0 => Eq_term s0
+  | app _ s0 s1 =>
+      congr_app (idSubst_term sigma_term Eq_term s0)
+        (idSubst_term sigma_term Eq_term s1)
+  | lam _ s0 =>
+      congr_lam
+        (idSubst_term (up_term_term sigma_term) (upId_term_term _ Eq_term) s0)
+  end.
+
+Lemma upExtRen_term_term {m : nat} {n : nat} (xi : fin m -> fin n)
+  (zeta : fin m -> fin n) (Eq : forall x, xi x = zeta x) :
+  forall x, upRen_term_term xi x = upRen_term_term zeta x.
+Proof.
+exact (fun n =>
+       match n with
+       | Some fin_n => ap shift (Eq fin_n)
+       | None => eq_refl
+       end).
+Qed.
+
+Lemma upExtRen_list_term_term {p : nat} {m : nat} {n : nat}
+  (xi : fin m -> fin n) (zeta : fin m -> fin n)
+  (Eq : forall x, xi x = zeta x) :
+  forall x, upRen_list_term_term p xi x = upRen_list_term_term p zeta x.
+Proof.
+exact (fun n =>
+       scons_p_congr (fun n => eq_refl) (fun n => ap (shift_p p) (Eq n))).
+Qed.
+
+Fixpoint extRen_term {m_term : nat} {n_term : nat}
+(xi_term : fin m_term -> fin n_term) (zeta_term : fin m_term -> fin n_term)
+(Eq_term : forall x, xi_term x = zeta_term x) (s : term m_term) {struct s} :
+ren_term xi_term s = ren_term zeta_term s :=
+  match s with
+  | var_term _ s0 => ap (var_term n_term) (Eq_term s0)
+  | app _ s0 s1 =>
+      congr_app (extRen_term xi_term zeta_term Eq_term s0)
+        (extRen_term xi_term zeta_term Eq_term s1)
+  | lam _ s0 =>
+      congr_lam
+        (extRen_term (upRen_term_term xi_term) (upRen_term_term zeta_term)
+           (upExtRen_term_term _ _ Eq_term) s0)
+  end.
+
+Lemma upExt_term_term {m : nat} {n_term : nat} (sigma : fin m -> term n_term)
+  (tau : fin m -> term n_term) (Eq : forall x, sigma x = tau x) :
+  forall x, up_term_term sigma x = up_term_term tau x.
+Proof.
+exact (fun n =>
+       match n with
+       | Some fin_n => ap (ren_term shift) (Eq fin_n)
+       | None => eq_refl
+       end).
+Qed.
+
+Lemma upExt_list_term_term {p : nat} {m : nat} {n_term : nat}
+  (sigma : fin m -> term n_term) (tau : fin m -> term n_term)
+  (Eq : forall x, sigma x = tau x) :
+  forall x, up_list_term_term p sigma x = up_list_term_term p tau x.
+Proof.
+exact (fun n =>
+       scons_p_congr (fun n => eq_refl)
+         (fun n => ap (ren_term (shift_p p)) (Eq n))).
+Qed.
+
+Fixpoint ext_term {m_term : nat} {n_term : nat}
+(sigma_term : fin m_term -> term n_term)
+(tau_term : fin m_term -> term n_term)
+(Eq_term : forall x, sigma_term x = tau_term x) (s : term m_term) {struct s}
+   : subst_term sigma_term s = subst_term tau_term s :=
+  match s with
+  | var_term _ s0 => Eq_term s0
+  | app _ s0 s1 =>
+      congr_app (ext_term sigma_term tau_term Eq_term s0)
+        (ext_term sigma_term tau_term Eq_term s1)
+  | lam _ s0 =>
+      congr_lam
+        (ext_term (up_term_term sigma_term) (up_term_term tau_term)
+           (upExt_term_term _ _ Eq_term) s0)
+  end.
+
+Lemma up_ren_ren_term_term {k : nat} {l : nat} {m : nat}
+  (xi : fin k -> fin l) (zeta : fin l -> fin m) (rho : fin k -> fin m)
+  (Eq : forall x, funcomp zeta xi x = rho x) :
+  forall x,
+  funcomp (upRen_term_term zeta) (upRen_term_term xi) x =
+  upRen_term_term rho x.
+Proof.
+exact (up_ren_ren xi zeta rho Eq).
+Qed.
+
+Lemma up_ren_ren_list_term_term {p : nat} {k : nat} {l : nat} {m : nat}
+  (xi : fin k -> fin l) (zeta : fin l -> fin m) (rho : fin k -> fin m)
+  (Eq : forall x, funcomp zeta xi x = rho x) :
+  forall x,
+  funcomp (upRen_list_term_term p zeta) (upRen_list_term_term p xi) x =
+  upRen_list_term_term p rho x.
+Proof.
+exact (up_ren_ren_p Eq).
+Qed.
+
+Fixpoint compRenRen_term {k_term : nat} {l_term : nat} {m_term : nat}
+(xi_term : fin m_term -> fin k_term) (zeta_term : fin k_term -> fin l_term)
+(rho_term : fin m_term -> fin l_term)
+(Eq_term : forall x, funcomp zeta_term xi_term x = rho_term x)
+(s : term m_term) {struct s} :
+ren_term zeta_term (ren_term xi_term s) = ren_term rho_term s :=
+  match s with
+  | var_term _ s0 => ap (var_term l_term) (Eq_term s0)
+  | app _ s0 s1 =>
+      congr_app (compRenRen_term xi_term zeta_term rho_term Eq_term s0)
+        (compRenRen_term xi_term zeta_term rho_term Eq_term s1)
+  | lam _ s0 =>
+      congr_lam
+        (compRenRen_term (upRen_term_term xi_term)
+           (upRen_term_term zeta_term) (upRen_term_term rho_term)
+           (up_ren_ren _ _ _ Eq_term) s0)
+  end.
+
+Lemma up_ren_subst_term_term {k : nat} {l : nat} {m_term : nat}
+  (xi : fin k -> fin l) (tau : fin l -> term m_term)
+  (theta : fin k -> term m_term) (Eq : forall x, funcomp tau xi x = theta x)
+  :
+  forall x,
+  funcomp (up_term_term tau) (upRen_term_term xi) x = up_term_term theta x.
+Proof.
+exact (fun n =>
+       match n with
+       | Some fin_n => ap (ren_term shift) (Eq fin_n)
+       | None => eq_refl
+       end).
+Qed.
+
+Lemma up_ren_subst_list_term_term {p : nat} {k : nat} {l : nat}
+  {m_term : nat} (xi : fin k -> fin l) (tau : fin l -> term m_term)
+  (theta : fin k -> term m_term) (Eq : forall x, funcomp tau xi x = theta x)
+  :
+  forall x,
+  funcomp (up_list_term_term p tau) (upRen_list_term_term p xi) x =
+  up_list_term_term p theta x.
+Proof.
+exact (fun n =>
+       eq_trans (scons_p_comp' _ _ _ n)
+         (scons_p_congr (fun z => scons_p_head' _ _ z)
+            (fun z =>
+             eq_trans (scons_p_tail' _ _ (xi z))
+               (ap (ren_term (shift_p p)) (Eq z))))).
+Qed.
+
+Fixpoint compRenSubst_term {k_term : nat} {l_term : nat} {m_term : nat}
+(xi_term : fin m_term -> fin k_term) (tau_term : fin k_term -> term l_term)
+(theta_term : fin m_term -> term l_term)
+(Eq_term : forall x, funcomp tau_term xi_term x = theta_term x)
+(s : term m_term) {struct s} :
+subst_term tau_term (ren_term xi_term s) = subst_term theta_term s :=
+  match s with
+  | var_term _ s0 => Eq_term s0
+  | app _ s0 s1 =>
+      congr_app (compRenSubst_term xi_term tau_term theta_term Eq_term s0)
+        (compRenSubst_term xi_term tau_term theta_term Eq_term s1)
+  | lam _ s0 =>
+      congr_lam
+        (compRenSubst_term (upRen_term_term xi_term) (up_term_term tau_term)
+           (up_term_term theta_term) (up_ren_subst_term_term _ _ _ Eq_term)
+           s0)
+  end.
+
+Lemma up_subst_ren_term_term {k : nat} {l_term : nat} {m_term : nat}
+  (sigma : fin k -> term l_term) (zeta_term : fin l_term -> fin m_term)
+  (theta : fin k -> term m_term)
+  (Eq : forall x, funcomp (ren_term zeta_term) sigma x = theta x) :
+  forall x,
+  funcomp (ren_term (upRen_term_term zeta_term)) (up_term_term sigma) x =
+  up_term_term theta x.
+Proof.
+exact (fun n =>
+       match n with
+       | Some fin_n =>
+           eq_trans
+             (compRenRen_term shift (upRen_term_term zeta_term)
+                (funcomp shift zeta_term) (fun x => eq_refl) (sigma fin_n))
+             (eq_trans
+                (eq_sym
+                   (compRenRen_term zeta_term shift (funcomp shift zeta_term)
+                      (fun x => eq_refl) (sigma fin_n)))
+                (ap (ren_term shift) (Eq fin_n)))
+       | None => eq_refl
+       end).
+Qed.
+
+Lemma up_subst_ren_list_term_term {p : nat} {k : nat} {l_term : nat}
+  {m_term : nat} (sigma : fin k -> term l_term)
+  (zeta_term : fin l_term -> fin m_term) (theta : fin k -> term m_term)
+  (Eq : forall x, funcomp (ren_term zeta_term) sigma x = theta x) :
+  forall x,
+  funcomp (ren_term (upRen_list_term_term p zeta_term))
+    (up_list_term_term p sigma) x = up_list_term_term p theta x.
+Proof.
+exact (fun n =>
+       eq_trans (scons_p_comp' _ _ _ n)
+         (scons_p_congr
+            (fun x => ap (var_term (plus p m_term)) (scons_p_head' _ _ x))
+            (fun n =>
+             eq_trans
+               (compRenRen_term (shift_p p)
+                  (upRen_list_term_term p zeta_term)
+                  (funcomp (shift_p p) zeta_term)
+                  (fun x => scons_p_tail' _ _ x) (sigma n))
+               (eq_trans
+                  (eq_sym
+                     (compRenRen_term zeta_term (shift_p p)
+                        (funcomp (shift_p p) zeta_term) (fun x => eq_refl)
+                        (sigma n))) (ap (ren_term (shift_p p)) (Eq n)))))).
+Qed.
+
+Fixpoint compSubstRen_term {k_term : nat} {l_term : nat} {m_term : nat}
+(sigma_term : fin m_term -> term k_term)
+(zeta_term : fin k_term -> fin l_term)
+(theta_term : fin m_term -> term l_term)
+(Eq_term : forall x, funcomp (ren_term zeta_term) sigma_term x = theta_term x)
+(s : term m_term) {struct s} :
+ren_term zeta_term (subst_term sigma_term s) = subst_term theta_term s :=
+  match s with
+  | var_term _ s0 => Eq_term s0
+  | app _ s0 s1 =>
+      congr_app
+        (compSubstRen_term sigma_term zeta_term theta_term Eq_term s0)
+        (compSubstRen_term sigma_term zeta_term theta_term Eq_term s1)
+  | lam _ s0 =>
+      congr_lam
+        (compSubstRen_term (up_term_term sigma_term)
+           (upRen_term_term zeta_term) (up_term_term theta_term)
+           (up_subst_ren_term_term _ _ _ Eq_term) s0)
+  end.
+
+Lemma up_subst_subst_term_term {k : nat} {l_term : nat} {m_term : nat}
+  (sigma : fin k -> term l_term) (tau_term : fin l_term -> term m_term)
+  (theta : fin k -> term m_term)
+  (Eq : forall x, funcomp (subst_term tau_term) sigma x = theta x) :
+  forall x,
+  funcomp (subst_term (up_term_term tau_term)) (up_term_term sigma) x =
+  up_term_term theta x.
+Proof.
+exact (fun n =>
+       match n with
+       | Some fin_n =>
+           eq_trans
+             (compRenSubst_term shift (up_term_term tau_term)
+                (funcomp (up_term_term tau_term) shift) (fun x => eq_refl)
+                (sigma fin_n))
+             (eq_trans
+                (eq_sym
+                   (compSubstRen_term tau_term shift
+                      (funcomp (ren_term shift) tau_term) (fun x => eq_refl)
+                      (sigma fin_n))) (ap (ren_term shift) (Eq fin_n)))
+       | None => eq_refl
+       end).
+Qed.
+
+Lemma up_subst_subst_list_term_term {p : nat} {k : nat} {l_term : nat}
+  {m_term : nat} (sigma : fin k -> term l_term)
+  (tau_term : fin l_term -> term m_term) (theta : fin k -> term m_term)
+  (Eq : forall x, funcomp (subst_term tau_term) sigma x = theta x) :
+  forall x,
+  funcomp (subst_term (up_list_term_term p tau_term))
+    (up_list_term_term p sigma) x = up_list_term_term p theta x.
+Proof.
+exact (fun n =>
+       eq_trans
+         (scons_p_comp' (funcomp (var_term (plus p l_term)) (zero_p p)) _ _ n)
+         (scons_p_congr
+            (fun x => scons_p_head' _ (fun z => ren_term (shift_p p) _) x)
+            (fun n =>
+             eq_trans
+               (compRenSubst_term (shift_p p) (up_list_term_term p tau_term)
+                  (funcomp (up_list_term_term p tau_term) (shift_p p))
+                  (fun x => eq_refl) (sigma n))
+               (eq_trans
+                  (eq_sym
+                     (compSubstRen_term tau_term (shift_p p) _
+                        (fun x => eq_sym (scons_p_tail' _ _ x)) (sigma n)))
+                  (ap (ren_term (shift_p p)) (Eq n)))))).
+Qed.
+
+Fixpoint compSubstSubst_term {k_term : nat} {l_term : nat} {m_term : nat}
+(sigma_term : fin m_term -> term k_term)
+(tau_term : fin k_term -> term l_term)
+(theta_term : fin m_term -> term l_term)
+(Eq_term : forall x,
+           funcomp (subst_term tau_term) sigma_term x = theta_term x)
+(s : term m_term) {struct s} :
+subst_term tau_term (subst_term sigma_term s) = subst_term theta_term s :=
+  match s with
+  | var_term _ s0 => Eq_term s0
+  | app _ s0 s1 =>
+      congr_app
+        (compSubstSubst_term sigma_term tau_term theta_term Eq_term s0)
+        (compSubstSubst_term sigma_term tau_term theta_term Eq_term s1)
+  | lam _ s0 =>
+      congr_lam
+        (compSubstSubst_term (up_term_term sigma_term)
+           (up_term_term tau_term) (up_term_term theta_term)
+           (up_subst_subst_term_term _ _ _ Eq_term) s0)
+  end.
+
+Lemma renRen_term {k_term : nat} {l_term : nat} {m_term : nat}
+  (xi_term : fin m_term -> fin k_term) (zeta_term : fin k_term -> fin l_term)
+  (s : term m_term) :
+  ren_term zeta_term (ren_term xi_term s) =
+  ren_term (funcomp zeta_term xi_term) s.
+Proof.
+exact (compRenRen_term xi_term zeta_term _ (fun n => eq_refl) s).
+Qed.
+
+Lemma renRen'_term_pointwise {k_term : nat} {l_term : nat} {m_term : nat}
+  (xi_term : fin m_term -> fin k_term) (zeta_term : fin k_term -> fin l_term)
+  :
+  pointwise_relation _ eq (funcomp (ren_term zeta_term) (ren_term xi_term))
+    (ren_term (funcomp zeta_term xi_term)).
+Proof.
+exact (fun s => compRenRen_term xi_term zeta_term _ (fun n => eq_refl) s).
+Qed.
+
+Lemma renSubst_term {k_term : nat} {l_term : nat} {m_term : nat}
+  (xi_term : fin m_term -> fin k_term) (tau_term : fin k_term -> term l_term)
+  (s : term m_term) :
+  subst_term tau_term (ren_term xi_term s) =
+  subst_term (funcomp tau_term xi_term) s.
+Proof.
+exact (compRenSubst_term xi_term tau_term _ (fun n => eq_refl) s).
+Qed.
+
+Lemma renSubst_term_pointwise {k_term : nat} {l_term : nat} {m_term : nat}
+  (xi_term : fin m_term -> fin k_term) (tau_term : fin k_term -> term l_term)
+  :
+  pointwise_relation _ eq (funcomp (subst_term tau_term) (ren_term xi_term))
+    (subst_term (funcomp tau_term xi_term)).
+Proof.
+exact (fun s => compRenSubst_term xi_term tau_term _ (fun n => eq_refl) s).
+Qed.
+
+Lemma substRen_term {k_term : nat} {l_term : nat} {m_term : nat}
+  (sigma_term : fin m_term -> term k_term)
+  (zeta_term : fin k_term -> fin l_term) (s : term m_term) :
+  ren_term zeta_term (subst_term sigma_term s) =
+  subst_term (funcomp (ren_term zeta_term) sigma_term) s.
+Proof.
+exact (compSubstRen_term sigma_term zeta_term _ (fun n => eq_refl) s).
+Qed.
+
+Lemma substRen_term_pointwise {k_term : nat} {l_term : nat} {m_term : nat}
+  (sigma_term : fin m_term -> term k_term)
+  (zeta_term : fin k_term -> fin l_term) :
+  pointwise_relation _ eq
+    (funcomp (ren_term zeta_term) (subst_term sigma_term))
+    (subst_term (funcomp (ren_term zeta_term) sigma_term)).
+Proof.
+exact (fun s => compSubstRen_term sigma_term zeta_term _ (fun n => eq_refl) s).
+Qed.
+
+Lemma substSubst_term {k_term : nat} {l_term : nat} {m_term : nat}
+  (sigma_term : fin m_term -> term k_term)
+  (tau_term : fin k_term -> term l_term) (s : term m_term) :
+  subst_term tau_term (subst_term sigma_term s) =
+  subst_term (funcomp (subst_term tau_term) sigma_term) s.
+Proof.
+exact (compSubstSubst_term sigma_term tau_term _ (fun n => eq_refl) s).
+Qed.
+
+Lemma substSubst_term_pointwise {k_term : nat} {l_term : nat} {m_term : nat}
+  (sigma_term : fin m_term -> term k_term)
+  (tau_term : fin k_term -> term l_term) :
+  pointwise_relation _ eq
+    (funcomp (subst_term tau_term) (subst_term sigma_term))
+    (subst_term (funcomp (subst_term tau_term) sigma_term)).
+Proof.
+exact (fun s =>
+       compSubstSubst_term sigma_term tau_term _ (fun n => eq_refl) s).
+Qed.
+
+Lemma rinstInst_up_term_term {m : nat} {n_term : nat}
+  (xi : fin m -> fin n_term) (sigma : fin m -> term n_term)
+  (Eq : forall x, funcomp (var_term n_term) xi x = sigma x) :
+  forall x,
+  funcomp (var_term (S n_term)) (upRen_term_term xi) x = up_term_term sigma x.
+Proof.
+exact (fun n =>
+       match n with
+       | Some fin_n => ap (ren_term shift) (Eq fin_n)
+       | None => eq_refl
+       end).
+Qed.
+
+Lemma rinstInst_up_list_term_term {p : nat} {m : nat} {n_term : nat}
+  (xi : fin m -> fin n_term) (sigma : fin m -> term n_term)
+  (Eq : forall x, funcomp (var_term n_term) xi x = sigma x) :
+  forall x,
+  funcomp (var_term (plus p n_term)) (upRen_list_term_term p xi) x =
+  up_list_term_term p sigma x.
+Proof.
+exact (fun n =>
+       eq_trans (scons_p_comp' _ _ (var_term (plus p n_term)) n)
+         (scons_p_congr (fun z => eq_refl)
+            (fun n => ap (ren_term (shift_p p)) (Eq n)))).
+Qed.
+
+Fixpoint rinst_inst_term {m_term : nat} {n_term : nat}
+(xi_term : fin m_term -> fin n_term) (sigma_term : fin m_term -> term n_term)
+(Eq_term : forall x, funcomp (var_term n_term) xi_term x = sigma_term x)
+(s : term m_term) {struct s} : ren_term xi_term s = subst_term sigma_term s
+:=
+  match s with
+  | var_term _ s0 => Eq_term s0
+  | app _ s0 s1 =>
+      congr_app (rinst_inst_term xi_term sigma_term Eq_term s0)
+        (rinst_inst_term xi_term sigma_term Eq_term s1)
+  | lam _ s0 =>
+      congr_lam
+        (rinst_inst_term (upRen_term_term xi_term) (up_term_term sigma_term)
+           (rinstInst_up_term_term _ _ Eq_term) s0)
+  end.
+
+Lemma rinstInst'_term {m_term : nat} {n_term : nat}
+  (xi_term : fin m_term -> fin n_term) (s : term m_term) :
+  ren_term xi_term s = subst_term (funcomp (var_term n_term) xi_term) s.
+Proof.
+exact (rinst_inst_term xi_term _ (fun n => eq_refl) s).
+Qed.
+
+Lemma rinstInst'_term_pointwise {m_term : nat} {n_term : nat}
+  (xi_term : fin m_term -> fin n_term) :
+  pointwise_relation _ eq (ren_term xi_term)
+    (subst_term (funcomp (var_term n_term) xi_term)).
+Proof.
+exact (fun s => rinst_inst_term xi_term _ (fun n => eq_refl) s).
+Qed.
+
+Lemma instId'_term {m_term : nat} (s : term m_term) :
+  subst_term (var_term m_term) s = s.
+Proof.
+exact (idSubst_term (var_term m_term) (fun n => eq_refl) s).
+Qed.
+
+Lemma instId'_term_pointwise {m_term : nat} :
+  pointwise_relation _ eq (subst_term (var_term m_term)) id.
+Proof.
+exact (fun s => idSubst_term (var_term m_term) (fun n => eq_refl) s).
+Qed.
+
+Lemma rinstId'_term {m_term : nat} (s : term m_term) : ren_term id s = s.
+Proof.
+exact (eq_ind_r (fun t => t = s) (instId'_term s) (rinstInst'_term id s)).
+Qed.
+
+Lemma rinstId'_term_pointwise {m_term : nat} :
+  pointwise_relation _ eq (@ren_term m_term m_term id) id.
+Proof.
+exact (fun s =>
+       eq_ind_r (fun t => t = s) (instId'_term s) (rinstInst'_term id s)).
+Qed.
+
+Lemma varL'_term {m_term : nat} {n_term : nat}
+  (sigma_term : fin m_term -> term n_term) (x : fin m_term) :
+  subst_term sigma_term (var_term m_term x) = sigma_term x.
+Proof.
+exact (eq_refl).
+Qed.
+
+Lemma varL'_term_pointwise {m_term : nat} {n_term : nat}
+  (sigma_term : fin m_term -> term n_term) :
+  pointwise_relation _ eq (funcomp (subst_term sigma_term) (var_term m_term))
+    sigma_term.
+Proof.
+exact (fun x => eq_refl).
+Qed.
+
+Lemma varLRen'_term {m_term : nat} {n_term : nat}
+  (xi_term : fin m_term -> fin n_term) (x : fin m_term) :
+  ren_term xi_term (var_term m_term x) = var_term n_term (xi_term x).
+Proof.
+exact (eq_refl).
+Qed.
+
+Lemma varLRen'_term_pointwise {m_term : nat} {n_term : nat}
+  (xi_term : fin m_term -> fin n_term) :
+  pointwise_relation _ eq (funcomp (ren_term xi_term) (var_term m_term))
+    (funcomp (var_term n_term) xi_term).
+Proof.
+exact (fun x => eq_refl).
+Qed.
+
+Class Up_term X Y :=
+    up_term : X -> Y.
+
+#[global]
+Instance Subst_term  {m_term n_term : nat}: (Subst1 _ _ _) :=
+ (@subst_term m_term n_term).
+
+#[global]
+Instance Up_term_term  {m n_term : nat}: (Up_term _ _) :=
+ (@up_term_term m n_term).
+
+#[global]
+Instance Ren_term  {m_term n_term : nat}: (Ren1 _ _ _) :=
+ (@ren_term m_term n_term).
+
+#[global]
+Instance VarInstance_term  {n_term : nat}: (Var _ _) := (@var_term n_term).
+
+Notation "[ sigma_term ]" := (subst_term sigma_term)
+( at level 1, left associativity, only printing)  : fscope.
+
+Notation "s [ sigma_term ]" := (subst_term sigma_term s)
+( at level 7, left associativity, only printing)  : subst_scope.
+
+Notation "↑__term" := up_term (only printing)  : subst_scope.
+
+Notation "↑__term" := up_term_term (only printing)  : subst_scope.
+
+Notation "⟨ xi_term ⟩" := (ren_term xi_term)
+( at level 1, left associativity, only printing)  : fscope.
+
+Notation "s ⟨ xi_term ⟩" := (ren_term xi_term s)
+( at level 7, left associativity, only printing)  : subst_scope.
+
+Notation "'var'" := var_term ( at level 1, only printing)  : subst_scope.
+
+Notation "x '__term'" := (@ids _ _ VarInstance_term x)
+( at level 5, format "x __term", only printing)  : subst_scope.
+
+Notation "x '__term'" := (var_term x) ( at level 5, format "x __term")  :
+subst_scope.
+
+#[global]
+Instance subst_term_morphism  {m_term : nat} {n_term : nat}:
+ (Proper (respectful (pointwise_relation _ eq) (respectful eq eq))
+    (@subst_term m_term n_term)).
+Proof.
+exact (fun f_term g_term Eq_term s t Eq_st =>
+       eq_ind s (fun t' => subst_term f_term s = subst_term g_term t')
+         (ext_term f_term g_term Eq_term s) t Eq_st).
+Qed.
+
+#[global]
+Instance subst_term_morphism2  {m_term : nat} {n_term : nat}:
+ (Proper (respectful (pointwise_relation _ eq) (pointwise_relation _ eq))
+    (@subst_term m_term n_term)).
+Proof.
+exact (fun f_term g_term Eq_term s => ext_term f_term g_term Eq_term s).
+Qed.
+
+#[global]
+Instance ren_term_morphism  {m_term : nat} {n_term : nat}:
+ (Proper (respectful (pointwise_relation _ eq) (respectful eq eq))
+    (@ren_term m_term n_term)).
+Proof.
+exact (fun f_term g_term Eq_term s t Eq_st =>
+       eq_ind s (fun t' => ren_term f_term s = ren_term g_term t')
+         (extRen_term f_term g_term Eq_term s) t Eq_st).
+Qed.
+
+#[global]
+Instance ren_term_morphism2  {m_term : nat} {n_term : nat}:
+ (Proper (respectful (pointwise_relation _ eq) (pointwise_relation _ eq))
+    (@ren_term m_term n_term)).
+Proof.
+exact (fun f_term g_term Eq_term s => extRen_term f_term g_term Eq_term s).
+Qed.
+
+Ltac auto_unfold := repeat
+                     unfold VarInstance_term, Var, ids, Ren_term, Ren1, ren1,
+                      Up_term_term, Up_term, up_term, Subst_term, Subst1,
+                      subst1.
+
+Tactic Notation "auto_unfold" "in" "*" := repeat
+                                           unfold VarInstance_term, Var, ids,
+                                            Ren_term, Ren1, ren1,
+                                            Up_term_term, Up_term, up_term,
+                                            Subst_term, Subst1, subst1 
+                                            in *.
+
+Ltac asimpl' := repeat (first
+                 [ progress setoid_rewrite substSubst_term_pointwise
+                 | progress setoid_rewrite substSubst_term
+                 | progress setoid_rewrite substRen_term_pointwise
+                 | progress setoid_rewrite substRen_term
+                 | progress setoid_rewrite renSubst_term_pointwise
+                 | progress setoid_rewrite renSubst_term
+                 | progress setoid_rewrite renRen'_term_pointwise
+                 | progress setoid_rewrite renRen_term
+                 | progress setoid_rewrite varLRen'_term_pointwise
+                 | progress setoid_rewrite varLRen'_term
+                 | progress setoid_rewrite varL'_term_pointwise
+                 | progress setoid_rewrite varL'_term
+                 | progress setoid_rewrite rinstId'_term_pointwise
+                 | progress setoid_rewrite rinstId'_term
+                 | progress setoid_rewrite instId'_term_pointwise
+                 | progress setoid_rewrite instId'_term
+                 | progress
+                    unfold up_list_term_term, up_term_term,
+                     upRen_list_term_term, upRen_term_term, up_ren
+                 | progress cbn[subst_term ren_term]
+                 | progress fsimpl ]).
+
+Ltac asimpl := check_no_evars;
+                repeat
+                 unfold VarInstance_term, Var, ids, Ren_term, Ren1, ren1,
+                  Up_term_term, Up_term, up_term, Subst_term, Subst1, subst1
+                  in *; asimpl'; minimize.
+
+Tactic Notation "asimpl" "in" hyp(J) := revert J; asimpl; intros J.
+
+Tactic Notation "auto_case" := auto_case ltac:(asimpl; cbn; eauto).
+
+Ltac substify := auto_unfold; try setoid_rewrite rinstInst'_term_pointwise;
+                  try setoid_rewrite rinstInst'_term.
+
+Ltac renamify := auto_unfold;
+                  try setoid_rewrite_left rinstInst'_term_pointwise;
+                  try setoid_rewrite_left rinstInst'_term.
+
+End Core.
+
+Module Extra.
+
+Import
+Core.
+
+Arguments var_term {n_term}.
+
+Arguments lam {n_term}.
+
+Arguments app {n_term}.
+
+#[global] Hint Opaque subst_term: rewrite.
+
+#[global] Hint Opaque ren_term: rewrite.
+
+End Extra.
+
+Module interface.
+
+Export Core.
+
+Export Extra.
+
+End interface.
+
+Export interface.
+
